feat: Separate counter examples from correct examples

examples/scalaEquivalenceBenchmarkExamples/incomplete/max2.dfy
@@ -32,22 +32,6 @@ lemma equivalenceMax1(l: List<int>)
   ensures (norm(l, max1(l)) == norm(l, maxM(l)))
 {}
 
-// CANDIDATE 2
-
-function max2(l: List<int>): int
-  decreases(l) {
-  match l
-    case Nil        => -999999999999 // represent very small number
-    case Cons(h, t) => if (h > max2(t)) then h else max2(t)
-}
-
-// In Stainless, max2 and maxM are equivalent if you replace -999999999999 with Int.MinValue
-// However, Dafny does not have a minimum integer constant, since integers are unbounded here
-// Therefore, Dafny cannot prove equivalence of max2 and maxM
-lemma equivalenceMax2(l: List<int>)
-  ensures (norm(l, max2(l)) == norm(l, maxM(l)))
-{}
-
 // CANDIDATE 3
 
 function length<T>(l: List<T>): nat
@@ -79,27 +63,3 @@ lemma equivalenceMax3(l: List<int>)
     case Cons(hd, Cons(hd1, tl1)) => assert length(Cons(hd, tl1)) < length(l);
     case _ =>
 }
-
-// CANDIDATE 4
-
-function max4(l: List<int>): int
-  decreases(l) {
-  match l {
-    case Nil          => 0
-    case Cons(hd, tl) => if (hd > max4(tl)) then hd else max4(tl)
-  }
-}
-
-// Counter example: l = Cons(-1, Nil)
-lemma equivalenceMax4(l: List<int>)
-  ensures (norm(l, max4(l)) == norm(l, maxM(l)))
-{}
-
-// CANDIDATE 5
-
-function max5(l: List<int>): int {-1}
-
-// Counter example: l = Cons(38, Nil)
-lemma equivalenceMax5(l: List<int>)
-  ensures (norm(l, max5(l)) == norm(l, maxM(l)))
-{}
