examples/scalaEquivalenceBenchmarkExamples/incomplete/counterExamples/max2CE.dfy
@@ -1,0 +1,58 @@
+// MODEL
+
+datatype List<T> = Nil | Cons(head: T, tail: List<T>)
+
+function maxM(lst: List<int>): int
+  decreases(lst) {
+  match lst {
+    case Nil             => -999999999999 // represent very small number
+    case Cons(hd, Nil)   => hd
+    case Cons(hd, tl)    => if (hd > maxM(tl)) then hd else maxM(tl)
+  }
+}
+
+function norm(l: List<int>, f: int): int {
+  match l
+    case Nil => -1
+    case _   => f
+}
+
+// CANDIDATE 2
+
+function max2(l: List<int>): int
+  decreases(l) {
+  match l
+    case Nil        => -999999999999 // represent very small number
+    case Cons(h, t) => if (h > max2(t)) then h else max2(t)
+}
+
+// In Stainless, max2 and maxM are equivalent if you replace -999999999999 with Int.MinValue
+// However, Dafny does not have a minimum integer constant, since integers are unbounded here
+// Therefore, Dafny cannot prove equivalence of max2 and maxM
+lemma equivalenceMax2(l: List<int>)
+  ensures (norm(l, max2(l)) == norm(l, maxM(l)))
+{}
+
+// CANDIDATE 4
+
+function max4(l: List<int>): int
+  decreases(l) {
+  match l {
+    case Nil          => 0
+    case Cons(hd, tl) => if (hd > max4(tl)) then hd else max4(tl)
+  }
+}
+
+// Counter example: l = Cons(-1, Nil)
+lemma equivalenceMax4(l: List<int>)
+  ensures (norm(l, max4(l)) == norm(l, maxM(l)))
+{}
+
+// CANDIDATE 5
+
+function max5(l: List<int>): int {-1}
+
+// Counter example: l = Cons(38, Nil)
+lemma equivalenceMax5(l: List<int>)
+  ensures (norm(l, max5(l)) == norm(l, maxM(l)))
+{}
