src/test/output/sigma.dfy
@@ -17,3 +17,9 @@ lemma sigmaM_sigma1_Equivalence(f: int -> int, a: int, b: int)
 ensures (sigmaM(f, a, b) == sigma1(f, a, b))
 {{}}
 
+lemma equivalenceSigmaRec_s(sum: int, i: int, b: int, f: int -> int)
+decreases (if (b == i) then 2 else if (b > i) then ((2 + b) - i) else (i - b))
+requires (i <= b)
+ensures (sigma_rec(sum, i, b, f) == s(i, b, f, sum))
+{{}}
+
