src/test/output/sorting.dfy
@@ -7,14 +7,6 @@ case Cons(x, xs) => loop(x, xs)
 }
 }
 
-function isSortedA(l: List<int>): bool
-{match l {
-case Nil => true
-case Cons(_, Nil) => true
-case Cons(x, Cons(y, ys)) => ((x <= y) && iter(Cons(y, ys)))
-}
-}
-
 function isSortedC(l: List<int>): bool
 {match l {
 case Nil => true
@@ -30,17 +22,6 @@ case Cons(x, Cons(y, ys)) => ((x <= y) && isSortedB(Cons(y, ys)))
 }
 }
 
-function iter(l: List<int>): bool
-{match l {
-case Nil => true
-case Cons(x, Nil) => true
-case Cons(x, Cons(y, ys)) => (leq(x, y) && iter(Cons(y, ys)))
-}
-}
-
-function leq(cur: int, next: int): bool
-{(cur < next)}
-
 function chk(l: List<int>, p: int, a: bool): bool
 {match l {
 case Nil => a
@@ -55,10 +36,6 @@ case Nil => true
 case Cons(x, xs) => ((p <= x) && loop(x, xs))
 }
 }
-
-lemma isSortedR_isSortedA_Equivalence(l: List<int>)
-ensures (isSortedR(l) == isSortedA(l))
-{{}}
 
 lemma isSortedR_isSortedC_Equivalence(l: List<int>)
 ensures (isSortedR(l) == isSortedC(l))
